x86/proofs/aes.ml
@@ -1,0 +1,123 @@
+(*
+ * Copyright Amazon.com, Inc. or its affiliates. All Rights Reserved.
+ * SPDX-License-Identifier: Apache-2.0 OR ISC OR MIT-0
+ *)
+
+(* References:
+   Intel 64 and IA-32 Architectures Software Developer's Manual Volume 1:
+     Basic Architecture, page 311-316
+   Intel 64 and IA-32 Architectures Software Developer's Manual Volume 2:
+     Instruction Set Reference, A-Z, 2A 3-63
+   White Paper: Intel Advanced Encryption Standard (AES) New Instructions Set *)
+
+let aesenc = new_definition
+ `aesenc (state:(128)word) (roundkey:(128)word) : (128)word =
+   let state = aes_shift_rows state in
+   let state = aes_sub_bytes joined_GF2 state in
+   let state = aes_mix_columns state in
+   (word_xor state roundkey)`;;
+
+let aesenclast = new_definition
+ `aesenclast (state:(128)word) (roundkey:(128)word) : (128)word =
+   let state = aes_shift_rows state in
+   let state = aes_sub_bytes joined_GF2 state in
+   (word_xor state roundkey)`;;
+
+let aesdec = new_definition
+ `aesdec (state:(128)word) (roundkey:(128)word) : (128)word =
+   let state = aes_inv_shift_rows state in
+   let state = aes_sub_bytes joined_GF2_inv state in
+   let state = aes_inv_mix_columns state in
+   (word_xor state roundkey)`;;
+
+let aesdeclast = new_definition
+ `aesdeclast (state:(128)word) (roundkey:(128)word) : (128)word =
+   let state = aes_inv_shift_rows state in
+   let state = aes_sub_bytes joined_GF2_inv state in
+   (word_xor state roundkey)`;;
+
+let aeskeygenassist = new_definition
+  `aeskeygenassist (x:(128)word) (imm8:(8)word) : (128)word =
+    let x3 = (word_subword:(128 word)->(num#num)->(32 word)) x (96,32) in
+    let x1 = (word_subword:(128 word)->(num#num)->(32 word)) x (32,32) in
+    let rcon = (word_zx:(8 word)->(32 word)) imm8 in
+    let dest0 = aes_subword x1 in
+    let dest1 = word_xor (aes_rotword (aes_subword x1)) rcon in
+    let dest2 = aes_subword x3 in
+    let dest3 = word_xor (aes_rotword (aes_subword x3)) rcon in
+    ((word_join:(32 word)->(96 word)->(128 word)) dest3
+     ((word_join:(32 word)->(64 word)->(96 word)) dest2
+      ((word_join:(32 word)->(32 word)->(64 word)) dest1 dest0)))`;;
+
+(************************************************)
+(** CONVERSIONS                                **)
+(************************************************)
+
+let AESENC_HELPER_CONV =
+  REWRITE_CONV [aesenc] THENC
+  AES_SHIFT_ROWS_CONV THENC
+  AES_SUB_BYTES_CONV THENC
+  AES_MIX_COLUMNS_CONV THENC
+  DEPTH_CONV (WORD_RED_CONV ORELSEC NUM_RED_CONV);;
+
+let AESENCLAST_HELPER_CONV =
+  REWRITE_CONV [aesenclast] THENC
+  AES_SHIFT_ROWS_CONV THENC
+  AES_SUB_BYTES_CONV THENC
+  DEPTH_CONV (WORD_RED_CONV ORELSEC NUM_RED_CONV);;
+
+let AESDEC_HELPER_CONV =
+  REWRITE_CONV [aesdec] THENC
+  AES_INV_SHIFT_ROWS_CONV THENC
+  AES_SUB_BYTES_CONV THENC
+  AES_INV_MIX_COLUMNS_CONV THENC
+  DEPTH_CONV (WORD_RED_CONV ORELSEC NUM_RED_CONV);;
+
+let AESDECLAST_HELPER_CONV =
+  REWRITE_CONV [aesdeclast] THENC
+  AES_INV_SHIFT_ROWS_CONV THENC
+  AES_SUB_BYTES_CONV THENC
+  DEPTH_CONV (WORD_RED_CONV ORELSEC NUM_RED_CONV);;
+
+let AESKEYGENASSIST_HELPER_CONV =
+  REWRITE_CONV [aeskeygenassist] THENC
+  AES_SUBWORD_CONV THENC
+  AES_ROTWORD_CONV THENC
+  TOP_DEPTH_CONV let_CONV THENC
+  DEPTH_CONV (WORD_RED_CONV ORELSEC NUM_RED_CONV);;
+
+let AESENC_REDUCE_CONV tm =
+  match tm with
+    Comb(Comb(Const("aesenc",_),
+         Comb(Const("word",_),state)),
+         Comb(Const("word",_),roundkey))
+    when is_numeral state && is_numeral roundkey -> AESENC_HELPER_CONV tm
+    | _ -> failwith "AESENC_REDUCE_CONV: inapplicable";;
+let AESENCLAST_REDUCE_CONV tm =
+  match tm with
+    Comb(Comb(Const("aesenclast",_),
+         Comb(Const("word",_),state)),
+         Comb(Const("word",_),roundkey))
+    when is_numeral state && is_numeral roundkey -> AESENCLAST_HELPER_CONV tm
+    | _ -> failwith "AESENCLAST_REDUCE_CONV: inapplicable";;
+let AESDEC_REDUCE_CONV tm =
+  match tm with
+    Comb(Comb(Const("aesdec",_),
+         Comb(Const("word",_),state)),
+         Comb(Const("word",_),roundkey))
+    when is_numeral state && is_numeral roundkey -> AESDEC_HELPER_CONV tm
+    | _ -> failwith "AESDEC_REDUCE_CONV: inapplicable";;
+let AESDECLAST_REDUCE_CONV tm =
+  match tm with
+    Comb(Comb(Const("aesdeclast",_),
+         Comb(Const("word",_),state)),
+         Comb(Const("word",_),roundkey))
+    when is_numeral state && is_numeral roundkey -> AESDECLAST_HELPER_CONV tm
+    | _ -> failwith "AESDECLAST_REDUCE_CONV: inapplicable";;
+let AESKEYGENASSIST_REDUCE_CONV tm =
+  match tm with
+    Comb(Comb(Const("aeskeygenassist",_),
+         Comb(Const("word",_),x)),
+         Comb(Const("word",_),imm8))
+    when is_numeral x && is_numeral imm8 -> AESKEYGENASSIST_HELPER_CONV tm
+    | _ -> failwith "AESKEYGENASSIST_HELPER_CONV: inapplicable";;
